arm/sha512/sha512_proofs.ml
@@ -1,370 +1,4 @@
-needs "arm/proofs/base.ml";;
-
-(* ------------------------------------------------------------------------- *)
-(* Mathematical specifications of SHA-512.                                   *)
-(* ------------------------------------------------------------------------- *)
-
-(*****************************************************************************)
-
-parse_as_prefix "~~";;
-override_interface("~~",`word_not:N word->N word`);;
-parse_as_infix("&&",(13,"right"));;
-override_interface("&&",`word_and:N word->N word->N word`);;
-parse_as_infix("||",(13,"right"));;
-override_interface("||",`word_or:N word->N word->N word`);;
-parse_as_infix("^^",(13,"right"));;
-override_interface("^^",`word_xor:N word->N word->N word`);;
-
-overload_interface("+",`word_add:N word->N word->N word`);;
-
-let Ch_DEF = new_definition
- `Ch(x,y,z):int64 = (x && y) ^^ (~~x && z)`;;
-
-let Maj_DEF = new_definition
- `Maj(x,y,z):int64 = (x && y) ^^ (x && z) ^^ (y && z)`;;
-
-let Sigma0_DEF = new_definition
- `Sigma0(x):int64 = word_ror x 28 ^^ word_ror x 34 ^^ word_ror x 39`;;
-
-let Sigma1_DEF = new_definition
- `Sigma1(x):int64 = word_ror x 14 ^^ word_ror x 18 ^^ word_ror x 41`;;
-
-let sigma0_DEF = new_definition
- `sigma0(x):int64 = word_ror x 1 ^^ word_ror x 8 ^^ word_ushr x 7`;;
-
-let sigma1_DEF = new_definition
- `sigma1(x):int64 = word_ror x 19 ^^ word_ror x 61 ^^ word_ushr x 6`;;
-
-unparse_as_prefix "~~";;
-remove_interface("~~");;
-unparse_as_infix("&&");;
-remove_interface("&&");;
-unparse_as_infix("||");;
-remove_interface("||");;
-unparse_as_infix("^^");;
-remove_interface("^^");;
-remove_interface("++");;
-
-(* ------------------------------------------------------------------------- *)
-(* Section 4.2.3                                                             *)
-(*                                                                           *)
-(* In principle these have a more concise mathematical definition            *)
-(* (first 64 fractional bit of cube roots of the first 80 primes)            *)
-(* but it's easier just to use them as magic numbers. This is copied         *)
-(* from TweetNaCl                                                            *)
-(* ------------------------------------------------------------------------- *)
-
-let  K_0  = new_definition  `K_0 : (64)word = word 0x428a2f98d728ae22`;;
-let  K_1  = new_definition  `K_1 : (64)word = word 0x7137449123ef65cd`;;
-let  K_2  = new_definition  `K_2 : (64)word = word 0xb5c0fbcfec4d3b2f`;;
-let  K_3  = new_definition  `K_3 : (64)word = word 0xe9b5dba58189dbbc`;;
-let  K_4  = new_definition  `K_4 : (64)word = word 0x3956c25bf348b538`;;
-let  K_5  = new_definition  `K_5 : (64)word = word 0x59f111f1b605d019`;;
-let  K_6  = new_definition  `K_6 : (64)word = word 0x923f82a4af194f9b`;;
-let  K_7  = new_definition  `K_7 : (64)word = word 0xab1c5ed5da6d8118`;;
-let  K_8  = new_definition  `K_8 : (64)word = word 0xd807aa98a3030242`;;
-let  K_9  = new_definition  `K_9 : (64)word = word 0x12835b0145706fbe`;;
-let K_10  = new_definition `K_10 : (64)word = word 0x243185be4ee4b28c`;;
-let K_11  = new_definition `K_11 : (64)word = word 0x550c7dc3d5ffb4e2`;;
-let K_12  = new_definition `K_12 : (64)word = word 0x72be5d74f27b896f`;;
-let K_13  = new_definition `K_13 : (64)word = word 0x80deb1fe3b1696b1`;;
-let K_14  = new_definition `K_14 : (64)word = word 0x9bdc06a725c71235`;;
-let K_15  = new_definition `K_15 : (64)word = word 0xc19bf174cf692694`;;
-let K_16  = new_definition `K_16 : (64)word = word 0xe49b69c19ef14ad2`;;
-let K_17  = new_definition `K_17 : (64)word = word 0xefbe4786384f25e3`;;
-let K_18  = new_definition `K_18 : (64)word = word 0x0fc19dc68b8cd5b5`;;
-let K_19  = new_definition `K_19 : (64)word = word 0x240ca1cc77ac9c65`;;
-let K_20  = new_definition `K_20 : (64)word = word 0x2de92c6f592b0275`;;
-let K_21  = new_definition `K_21 : (64)word = word 0x4a7484aa6ea6e483`;;
-let K_22  = new_definition `K_22 : (64)word = word 0x5cb0a9dcbd41fbd4`;;
-let K_23  = new_definition `K_23 : (64)word = word 0x76f988da831153b5`;;
-let K_24  = new_definition `K_24 : (64)word = word 0x983e5152ee66dfab`;;
-let K_25  = new_definition `K_25 : (64)word = word 0xa831c66d2db43210`;;
-let K_26  = new_definition `K_26 : (64)word = word 0xb00327c898fb213f`;;
-let K_27  = new_definition `K_27 : (64)word = word 0xbf597fc7beef0ee4`;;
-let K_28  = new_definition `K_28 : (64)word = word 0xc6e00bf33da88fc2`;;
-let K_29  = new_definition `K_29 : (64)word = word 0xd5a79147930aa725`;;
-let K_30  = new_definition `K_30 : (64)word = word 0x06ca6351e003826f`;;
-let K_31  = new_definition `K_31 : (64)word = word 0x142929670a0e6e70`;;
-let K_32  = new_definition `K_32 : (64)word = word 0x27b70a8546d22ffc`;;
-let K_33  = new_definition `K_33 : (64)word = word 0x2e1b21385c26c926`;;
-let K_34  = new_definition `K_34 : (64)word = word 0x4d2c6dfc5ac42aed`;;
-let K_35  = new_definition `K_35 : (64)word = word 0x53380d139d95b3df`;;
-let K_36  = new_definition `K_36 : (64)word = word 0x650a73548baf63de`;;
-let K_37  = new_definition `K_37 : (64)word = word 0x766a0abb3c77b2a8`;;
-let K_38  = new_definition `K_38 : (64)word = word 0x81c2c92e47edaee6`;;
-let K_39  = new_definition `K_39 : (64)word = word 0x92722c851482353b`;;
-let K_40  = new_definition `K_40 : (64)word = word 0xa2bfe8a14cf10364`;;
-let K_41  = new_definition `K_41 : (64)word = word 0xa81a664bbc423001`;;
-let K_42  = new_definition `K_42 : (64)word = word 0xc24b8b70d0f89791`;;
-let K_43  = new_definition `K_43 : (64)word = word 0xc76c51a30654be30`;;
-let K_44  = new_definition `K_44 : (64)word = word 0xd192e819d6ef5218`;;
-let K_45  = new_definition `K_45 : (64)word = word 0xd69906245565a910`;;
-let K_46  = new_definition `K_46 : (64)word = word 0xf40e35855771202a`;;
-let K_47  = new_definition `K_47 : (64)word = word 0x106aa07032bbd1b8`;;
-let K_48  = new_definition `K_48 : (64)word = word 0x19a4c116b8d2d0c8`;;
-let K_49  = new_definition `K_49 : (64)word = word 0x1e376c085141ab53`;;
-let K_50  = new_definition `K_50 : (64)word = word 0x2748774cdf8eeb99`;;
-let K_51  = new_definition `K_51 : (64)word = word 0x34b0bcb5e19b48a8`;;
-let K_52  = new_definition `K_52 : (64)word = word 0x391c0cb3c5c95a63`;;
-let K_53  = new_definition `K_53 : (64)word = word 0x4ed8aa4ae3418acb`;;
-let K_54  = new_definition `K_54 : (64)word = word 0x5b9cca4f7763e373`;;
-let K_55  = new_definition `K_55 : (64)word = word 0x682e6ff3d6b2b8a3`;;
-let K_56  = new_definition `K_56 : (64)word = word 0x748f82ee5defb2fc`;;
-let K_57  = new_definition `K_57 : (64)word = word 0x78a5636f43172f60`;;
-let K_58  = new_definition `K_58 : (64)word = word 0x84c87814a1f0ab72`;;
-let K_59  = new_definition `K_59 : (64)word = word 0x8cc702081a6439ec`;;
-let K_60  = new_definition `K_60 : (64)word = word 0x90befffa23631e28`;;
-let K_61  = new_definition `K_61 : (64)word = word 0xa4506cebde82bde9`;;
-let K_62  = new_definition `K_62 : (64)word = word 0xbef9a3f7b2c67915`;;
-let K_63  = new_definition `K_63 : (64)word = word 0xc67178f2e372532b`;;
-let K_64  = new_definition `K_64 : (64)word = word 0xca273eceea26619c`;;
-let K_65  = new_definition `K_65 : (64)word = word 0xd186b8c721c0c207`;;
-let K_66  = new_definition `K_66 : (64)word = word 0xeada7dd6cde0eb1e`;;
-let K_67  = new_definition `K_67 : (64)word = word 0xf57d4f7fee6ed178`;;
-let K_68  = new_definition `K_68 : (64)word = word 0x06f067aa72176fba`;;
-let K_69  = new_definition `K_69 : (64)word = word 0x0a637dc5a2c898a6`;;
-let K_70  = new_definition `K_70 : (64)word = word 0x113f9804bef90dae`;;
-let K_71  = new_definition `K_71 : (64)word = word 0x1b710b35131c471b`;;
-let K_72  = new_definition `K_72 : (64)word = word 0x28db77f523047d84`;;
-let K_73  = new_definition `K_73 : (64)word = word 0x32caab7b40c72493`;;
-let K_74  = new_definition `K_74 : (64)word = word 0x3c9ebe0a15c9bebc`;;
-let K_75  = new_definition `K_75 : (64)word = word 0x431d67c49c100d4c`;;
-let K_76  = new_definition `K_76 : (64)word = word 0x4cc5d4becb3e42b6`;;
-let K_77  = new_definition `K_77 : (64)word = word 0x597f299cfc657e2a`;;
-let K_78  = new_definition `K_78 : (64)word = word 0x5fcb6fab3ad6faec`;;
-let K_79  = new_definition `K_79 : (64)word = word 0x6c44198c4a475817`;;
-
-let ktbl_list = new_definition `ktbl_list : ((64)word)list =
-              [  K_0;  K_1;  K_2;  K_3;  K_4;  K_5;  K_6;  K_7;  K_8;  K_9;
-                 K_10; K_11; K_12; K_13; K_14; K_15; K_16; K_17; K_18; K_19;
-                 K_20; K_21; K_22; K_23; K_24; K_25; K_26; K_27; K_28; K_29;
-                 K_30; K_31; K_32; K_33; K_34; K_35; K_36; K_37; K_38; K_39;
-                 K_40; K_41; K_42; K_43; K_44; K_45; K_46; K_47; K_48; K_49;
-                 K_50; K_51; K_52; K_53; K_54; K_55; K_56; K_57; K_58; K_59;
-                 K_60; K_61; K_62; K_63; K_64; K_65; K_66; K_67; K_68; K_69;
-                 K_70; K_71; K_72; K_73; K_74; K_75; K_76; K_77; K_78; K_79 ]`;;
-
-let K_DEF = new_definition `K i:int64 = EL i ktbl_list`;;
-
-(* ------------------------------------------------------------------------- *)
-(* Section 5.3.5: the initial value of the 8 hash variables.                 *)
-(* ------------------------------------------------------------------------- *)
-
-let h_a = new_definition `h_a : (64)word = word 0x6a09e667f3bcc908`;;
-let h_b = new_definition `h_b : (64)word = word 0xbb67ae8584caa73b`;;
-let h_c = new_definition `h_c : (64)word = word 0x3c6ef372fe94f82b`;;
-let h_d = new_definition `h_d : (64)word = word 0xa54ff53a5f1d36f1`;; 
-let h_e = new_definition `h_e : (64)word = word 0x510e527fade682d1`;;
-let h_f = new_definition `h_f : (64)word = word 0x9b05688c2b3e6c1f`;;
-let h_g = new_definition `h_g : (64)word = word 0x1f83d9abfb41bd6b`;; 
-let h_h = new_definition `h_h : (64)word = word 0x5be0cd19137e2179`;;
-
-new_type_abbrev("hash_t",`:int64#int64#int64#int64#int64#int64#int64#int64`);;
-
-let h_init = new_definition
-  `h_init : hash_t = h_a, h_b, h_c, h_d, h_e, h_f, h_g, h_h`;;
-
-(* ------------------------------------------------------------------------- *)
-(* Main inner loop iteration.                                                *)
-(* ------------------------------------------------------------------------- *)
-
-let msg_schedule_word = define
-  `msg_schedule_word w1 w2 w3 w4 =
-    sigma1 w1 + w2 + sigma0 w3 + w4`;;
-
-let msg_schedule = define
- `msg_schedule (m:num->int64) (i:num) : int64 =
-      if i < 16 then word_bytereverse (m i)
-      else msg_schedule_word (msg_schedule m (i - 2))
-                                 (msg_schedule m (i - 7))
-                                 (msg_schedule m (i - 15))
-                                 (msg_schedule m (i - 16))`;;
-
-let compression_t1 = define
-  `compression_t1 e f g h = h + Sigma1(e) + Ch(e,f,g)`;;
-
-let compression_t2 = define
-  `compression_t2 a b c = Sigma0(a) + Maj(a,b,c)`;;
-
-let SHA512_A = define 
-  `SHA512_A(a:int64,b:int64,c:int64,d:int64,e:int64,f:int64,g:int64,h:int64) = a`;;
-let SHA512_B = define 
-  `SHA512_B(a:int64,b:int64,c:int64,d:int64,e:int64,f:int64,g:int64,h:int64) = b`;;
-let SHA512_C = define 
-  `SHA512_C(a:int64,b:int64,c:int64,d:int64,e:int64,f:int64,g:int64,h:int64) = c`;;
-let SHA512_D = define 
-  `SHA512_D(a:int64,b:int64,c:int64,d:int64,e:int64,f:int64,g:int64,h:int64) = d`;;
-let SHA512_E = define 
-  `SHA512_E(a:int64,b:int64,c:int64,d:int64,e:int64,f:int64,g:int64,h:int64) = e`;;
-let SHA512_F = define 
-  `SHA512_F(a:int64,b:int64,c:int64,d:int64,e:int64,f:int64,g:int64,h:int64) = f`;;
-let SHA512_G = define 
-  `SHA512_G(a:int64,b:int64,c:int64,d:int64,e:int64,f:int64,g:int64,h:int64) = g`;;
-let SHA512_H = define 
-  `SHA512_H(a:int64,b:int64,c:int64,d:int64,e:int64,f:int64,g:int64,h:int64) = h`;;
-
-let compression_update = define
- `compression_update hash ki wi =
-    let a = SHA512_A hash in
-    let b = SHA512_B hash in
-    let c = SHA512_C hash in
-    let d = SHA512_D hash in
-    let e = SHA512_E hash in
-    let f = SHA512_F hash in
-    let g = SHA512_G hash in
-    let h = SHA512_H hash in
-    let t1 = (compression_t1 e f g h) + ki + wi in
-    let t2 = compression_t2 a b c in
-    (t1 + t2, a, b, c, d + t1, e, f, g)`;;
-      
-let compression = define
-  `compression (i:num) hash (m:num->int64) =
-      if i < 80 then
-        let ki = K i in
-        let wi = msg_schedule m i in
-        let update = compression_update hash (K i) wi in
-        compression (i + 1) update m
-      else 
-        hash`;;
-
-let add8 = define 
- `add8 hash hash' = 
-  let a = SHA512_A hash in
-  let b = SHA512_B hash in
-  let c = SHA512_C hash in
-  let d = SHA512_D hash in
-  let e = SHA512_E hash in
-  let f = SHA512_F hash in
-  let g = SHA512_G hash in
-  let h = SHA512_H hash in
-  let a' = SHA512_A hash' in
-  let b' = SHA512_B hash' in
-  let c' = SHA512_C hash' in
-  let d' = SHA512_D hash' in
-  let e' = SHA512_E hash' in
-  let f' = SHA512_F hash' in
-  let g' = SHA512_G hash' in
-  let h' = SHA512_H hash' in
-  (a+a',b+b',c+c',d+d',e+e',f+f',g+g',h+h')`;;
-
-let sha512_block = define
- `sha512_block (m:num->int64) hash =
-    let hash' = compression 0 hash m in
-    add8 hash' hash`;;
-
-let sha512' = define
-  `sha512' hash (m:num->num->int64) (i:num) =
-    if i = 0 then hash
-    else sha512_block (m (i - 1)) (sha512' hash m (i - 1))`;;
-
-let sha512 = define 
-  `sha512 = sha512' h_init`;;
-
-let num_bytes_per_block = define
-  `num_bytes_per_block = 128`;;
-
-let ceil_div = define
-  `ceil_div (m : num) (n : num) = (m + n - 1) DIV n`;;
-
-parse_as_infix ("++", (13, "right"));;
-override_interface("++", `APPEND`);;
-
-let int128_to_bytes = define
-  `int128_to_bytes (w : int128) : byte list =
-    [word_subword w (0, 8); word_subword w (8, 8);
-     word_subword w (16, 8); word_subword w (24, 8);
-     word_subword w (32, 8); word_subword w (40, 8);
-     word_subword w (48, 8); word_subword w (56, 8);
-     word_subword w (64, 8); word_subword w (72, 8);
-     word_subword w (80, 8); word_subword w (88, 8);
-     word_subword w (96, 8); word_subword w (104, 8);
-     word_subword w (112, 8); word_subword w (120, 8)]`;;
-
-(* Pad a message with 100...0<l> until it is a multiple of blocks,
- * where l is a 128-bit big-endian word equal to the number of bits in the message *)
-let pad = define
-  `pad (m : byte list) : byte list = m ++ [word 0x80] ++
-    REPLICATE ((ceil_div (LENGTH m + 1 + 16) num_bytes_per_block) * num_bytes_per_block - (LENGTH m + 1 + 16)) (word 0) ++
-    int128_to_bytes (word_bytereverse (word (LENGTH m * 8)))`;;
-
-let take = define
-  `take (n : num) (l : A list) : A list =
-    SUB_LIST (0, n) l`;;
-
-let drop = define
-  `drop (n : num) (l : A list) : A list =
-    SUB_LIST (n, LENGTH l - n) l`;;
-
-let join_bytes_to_int64 = define
-  `join_bytes_to_int64  (bs : byte list) : int64 =
-    word_join
-      (word_join (word_join (EL 7 bs) (EL 6 bs) : int16) (word_join (EL 5 bs) (EL 4 bs) : int16) : int32)
-      (word_join (word_join (EL 3 bs) (EL 2 bs) : int16) (word_join (EL 1 bs) (EL 0 bs) : int16) : int32)`;;
-
-(* Conversion from byte list to a block of 8-byte words *)
-let bytes_to_one_block = define
-  `bytes_to_one_block (m : byte list) : num -> int64 =
-    \i. join_bytes_to_int64 (SUB_LIST (i * 8, 8) m)`;;
-
-(* Conversion from byte list to blocks of 8-byte words *)
-let bytes_to_blocks = define
-  `bytes_to_blocks (m : byte list) : num -> num -> int64 =
-    \i. bytes_to_one_block (SUB_LIST (i * num_bytes_per_block, num_bytes_per_block) m)`;;
-
-let bytes_mod_blocks = define
-  `bytes_mod_blocks (m : byte list) : byte list =
-    drop ((LENGTH m DIV num_bytes_per_block) * num_bytes_per_block) m`;;
-
-let sha512_ctx_from = define
-  `sha512_ctx_from (m : byte list) =
-    (sha512 (bytes_to_blocks m) (LENGTH m DIV num_bytes_per_block),
-     word ((LENGTH m * 8) MOD (2 EXP 64)) : int64, word ((LENGTH m * 8) DIV (2 EXP 64)) : int64,
-     bytes_mod_blocks m)`;;
-
-(*****************************************************************************)
-
-(* ------------------------------------------------------------------------- *)
-(* Auxiliary definitions to associate memory contents with HOL Light terms.  *)
-(* ------------------------------------------------------------------------- *)
-
-(*****************************************************************************)
-
-let hash_buffer_at = define
-  `hash_buffer_at (h : hash_t) (h_p : int64) s =
-    (read (memory :> bytes64(h_p)) s,                          read (memory :> bytes64 (word_add h_p (word 8))) s,
-     read (memory :> bytes64 (word_add h_p (word (8 * 2)))) s, read (memory :> bytes64 (word_add h_p (word (8 * 3)))) s,
-     read (memory :> bytes64 (word_add h_p (word (8 * 4)))) s, read (memory :> bytes64 (word_add h_p (word (8 * 5)))) s,
-     read (memory :> bytes64 (word_add h_p (word (8 * 6)))) s, read (memory :> bytes64 (word_add h_p (word (8 * 7)))) s) = h`;;
-
-let byte_list_at = define
-  `byte_list_at (m : byte list) (l : num) (m_p : int64) s =
-    (LENGTH m = l /\
-     ! i. i < l ==> read (memory :> bytes8(word_add m_p (word i))) s = EL i m)`;;
-
-let msg_block_at = define
-  `msg_block_at (m : num -> int64) (m_p : int64) s =
-    (read (memory :> bytes64(m_p)) s = m 0                            /\ read (memory :> bytes64(word_add m_p (word 8))) s = m 1 /\
-     read (memory :> bytes64(word_add m_p (word (8 * 2)))) s = m 2    /\ read (memory :> bytes64(word_add m_p (word (8 * 3)))) s = m 3 /\
-     read (memory :> bytes64(word_add m_p (word (8 * 4)))) s = m 4    /\ read (memory :> bytes64(word_add m_p (word (8 * 5)))) s = m 5 /\
-     read (memory :> bytes64(word_add m_p (word (8 * 6)))) s = m 6    /\ read (memory :> bytes64(word_add m_p (word (8 * 7)))) s = m 7 /\
-     read (memory :> bytes64(word_add m_p (word (8 * 8)))) s = m 8    /\ read (memory :> bytes64(word_add m_p (word (8 * 9)))) s = m 9 /\
-     read (memory :> bytes64(word_add m_p (word (8 * 10)))) s = m 10  /\ read (memory :> bytes64(word_add m_p (word (8 * 11)))) s = m 11 /\
-     read (memory :> bytes64(word_add m_p (word (8 * 12)))) s = m 12  /\ read (memory :> bytes64(word_add m_p (word (8 * 13)))) s = m 13 /\
-     read (memory :> bytes64(word_add m_p (word (8 * 14)))) s = m 14  /\ read (memory :> bytes64(word_add m_p (word (8 * 15)))) s = m 15)`;;
-
-let msg_blocks_at = define
-  `msg_blocks_at (m : num -> num -> int64) (l : num) (m_p : int64) s =
-    ! i. i < l ==> msg_block_at (m i) (word_add m_p (word (num_bytes_per_block * i))) s`;;
-
-let sha512_ctx_at = define
-  `sha512_ctx_at (m : byte list) (ctx_p : int64) s =
-    let h, msg_len_lo, msg_len_hi, cur_block = sha512_ctx_from m in
-    (hash_buffer_at h ctx_p s /\
-     read (memory :> bytes64 (word_add ctx_p (word (8 * 8)))) s = msg_len_lo /\
-     read (memory :> bytes64 (word_add ctx_p (word (8 * 9)))) s = msg_len_hi /\
-     take (LENGTH cur_block) (read (memory :> bytelist (word_add ctx_p (word (8 * 10)), num_bytes_per_block)) s) = cur_block /\
-     read (memory :> bytes8 (word_add ctx_p (word 208))) s = word (LENGTH cur_block))`;;
+needs "arm/sha512/sha512_specs.ml";;
 
 (*****************************************************************************)
 
@@ -1088,14 +722,14 @@ let a_mc,a_constants_data = define_assert_relocs_from_elf "a_mc"
 let EXEC = ARM_MK_EXEC_RULE a_mc;;
 
 (* sha512_init *)
-let SHA512_INIT = prove(`! ctx_p pc retpc K.
+let SHA512_INIT = prove(`! ctx_p pc retpc K_base.
   nonoverlapping (word pc : int64, 2748) (ctx_p, 216) ==>
   ensures arm
-    (\s. aligned_bytes_loaded s (word pc) (a_mc pc K) /\
+    (\s. aligned_bytes_loaded s (word pc) (a_mc pc K_base) /\
          read PC s = word (pc + 0x2b0) /\
-         read X30 s = retpc /\
+         read X30 s = word retpc /\
          read X0 s = ctx_p)
-    (\s. read PC s = retpc /\
+    (\s. read PC s = word retpc /\
          sha512_ctx_at [] ctx_p s)
     (MAYCHANGE [X1; X2; X3; X4; X5; X6; X7; PC] ,,
      MAYCHANGE [memory :> bytes(ctx_p, 216)] ,, MAYCHANGE [events])`,
@@ -1123,23 +757,23 @@ let FORALL_LT_SUC = prove
   REWRITE_TAC[GSYM ADD1] THEN MESON_TAC[LT]);;
 
 (* msg_schedule *)
-let MSG_SCHEDULE = prove(`! sch_p m_p m pc retpc K.
+let MSG_SCHEDULE = prove(`! sch_p m_p m pc retpc K_base.
   PAIRWISE nonoverlapping
     [(word pc : int64, 2748); (sch_p, 640); (m_p, num_bytes_per_block)] ==>
   ensures arm
-    (\s. aligned_bytes_loaded s (word pc) (a_mc pc K) /\
+    (\s. aligned_bytes_loaded s (word pc) (a_mc pc K_base) /\
          read PC s = word pc /\
          read X30 s = word retpc /\
          read X0 s = sch_p /\ 
          read X1 s = m_p /\
          msg_block_at m m_p s)
     (\s. read PC s = word retpc /\
-         ! i. i < 80 ==> read (memory :> bytes64(word_add sch_p (word (8 * i)))) s = msg_schedule m i)
+         msg_schedule_at m sch_p s)
     (MAYCHANGE [X0; X1; X2; X3; X4; X5; X6; X7; X8; X9; X10; X11; PC] ,,
      MAYCHANGE [memory :> bytes(sch_p, 640)] ,, MAYCHANGE SOME_FLAGS ,,
      MAYCHANGE [events])`,
-  REWRITE_TAC[SOME_FLAGS] THEN
-  REWRITE_TAC[NONOVERLAPPING_CLAUSES; PAIRWISE; ALL; num_bytes_per_block] THEN
+  REWRITE_TAC[SOME_FLAGS; NONOVERLAPPING_CLAUSES; PAIRWISE; ALL;
+              num_bytes_per_block; msg_schedule_at] THEN
   REPEAT STRIP_TAC THEN
   ENSURES_WHILE_UP_TAC
     `16` `pc + 0x4` `pc + 0x58`
@@ -1258,15 +892,28 @@ let MSG_SCHEDULE = prove(`! sch_p m_p m pc retpc K.
   ARM_SIM_TAC EXEC (51--53) THEN
   CHEAT_TAC);;
 
+(* let EXPAND_HASH = prove(`! h : hash_t. h =
+(SHA512_A h, SHA512_B h, SHA512_C h, SHA512_D h,
+ SHA512_E h, SHA512_F h, SHA512_G h, SHA512_H h)`,
+REWRITE_TAC [FORALL_PAIR_THM; PAIR_EQ; SHA512_A; SHA512_B; SHA512_C;
+SHA512_D; SHA512_E; SHA512_F; SHA512_G; SHA512_H]);; *)
 
 
+let EXPAND_HASH_THM = prove(
+  `! h0 h1 h2 h3 h4 h5 h6 h7 h.
+    (h0, h1, h2, h3, h4, h5, h6, h7) = h <=>
+      h0 = SHA512_A h /\ h1 = SHA512_B h /\
+      h2 = SHA512_C h /\ h3 = SHA512_D h /\
+      h4 = SHA512_E h /\ h5 = SHA512_F h /\
+      h6 = SHA512_G h /\ h7 = SHA512_H h`,
+  REWRITE_TAC [FORALL_PAIR_THM; PAIR_EQ; SHA512_A; SHA512_B; SHA512_C;
+    SHA512_D; SHA512_E; SHA512_F; SHA512_G; SHA512_H]);;
 
 
-
-
-
-
-     
+let RENAME_TAC old_name new_name =
+POP_ASSUM_LIST(MP_TAC o end_itlist CONJ o rev) THEN
+SPEC_TAC(old_name, new_name) THEN 
+STRIP_TAC THEN STRIP_TAC;;
 
 
 
@@ -1276,21 +923,22 @@ let MSG_SCHEDULE = prove(`! sch_p m_p m pc retpc K.
 let rec back_up n = if n > 1 then (b(); back_up (n-1)) else b();;
 
 (* void sha512_process_block(uint64_t h[8], const uint8_t *in_data) *)
-g `! sp h_p h m_p m pc retpc K.
+g `! sp h_p h m_p m pc retpc K_base.
+  aligned 16 sp /\
+  adrp_within_bounds (word K_base) (word (pc + 0x120)) /\
   PAIRWISE nonoverlapping
     [(word pc : int64, 2748); (h_p, 64);
      (m_p, num_bytes_per_block); (word_sub sp (word 720), 720)] ==>
     ensures arm
-    (\s. aligned_bytes_loaded s (word pc) (a_mc pc K) /\
+    (\s. aligned_bytes_loaded s (word pc) (a_mc pc K_base) /\
          read PC s = word (pc + 0xe0) /\
-         read X30 s = retpc /\
+         read X30 s = word retpc /\
          read SP s = sp /\
-         aligned 16 sp /\
          read X0 s = h_p /\
          read X1 s = m_p /\
          hash_buffer_at h h_p s /\
          msg_block_at m m_p s)
-    (\s. read PC s = retpc /\
+    (\s. read PC s = word retpc /\
          hash_buffer_at (sha512_block m h) h_p s)
     (MAYCHANGE [X0; X1; X2; X3; X4; X5; X6; X7; X8; X9; X10; X11;
                 X12; X13; X14; X15; X16; X17; X18; PC] ,,
@@ -1298,31 +946,126 @@ g `! sp h_p h m_p m pc retpc K.
      MAYCHANGE [memory :> bytes(word_sub sp (word 720), 720)] ,,
      MAYCHANGE SOME_FLAGS ,, MAYCHANGE [events])`;;
 
-e (REWRITE_TAC[SOME_FLAGS; NONOVERLAPPING_CLAUSES; PAIRWISE; ALL; num_bytes_per_block]);;
-e (WORD_FORALL_OFFSET_TAC 720);;
-e (REPEAT STRIP_TAC);;
-e (ENSURES_EXISTING_PRESERVED_TAC `SP`);;
-e (ENSURES_PRESERVED_TAC "x29_init" `X29`);;
-e (ENSURES_EXISTING_PRESERVED_TAC `X30`);;
+REWRITE_TAC[SOME_FLAGS; NONOVERLAPPING_CLAUSES; PAIRWISE; ALL; num_bytes_per_block] THEN
+WORD_FORALL_OFFSET_TAC 720 THEN
+REPEAT STRIP_TAC THEN
+ENSURES_EXISTING_PRESERVED_TAC `SP` THEN
+ENSURES_PRESERVED_TAC "x29_init" `X29` THEN
+ENSURES_EXISTING_PRESERVED_TAC `X30` THEN
 
-e (ENSURES_INIT_TAC "s56");;
-e (ARM_STEPS_TAC EXEC (57--61));;
+ENSURES_WHILE_UP_TAC
+  `79` `pc + 0x158` `pc + 0x158`
+  `\i s. // loop invariant
+    (read (memory :> bytes64(sp)) s = x29_init /\
+    read (memory :> bytes64(sp + word 8)) s = word retpc /\
+    read X12 s = h_p /\
+    read X14 s = K_base /\ read X6 s = word (i + 1) /\
+  (read X5 s, read X8 s, read X7 s, read X13 s,
+      read X3 s, read X10 s, read X9 s, read X11 s) =
+      compression_until i 0 h m /\
+    msg_schedule_at m (sp + word 0x50) s /\
+    hash_buffer_at h h_p s)` THEN
+REPEAT CONJ_TAC THENL
 
+[ (* Subgoal 1: upper bound of counter is non-zero *)
+  ARITH_TAC;
+   ;
+  ;
+  ;
+  ;
+]
+  (* Subgoal 2: initialization *)
+  REWRITE_TAC [msg_block_at; hash_buffer_at; EXPAND_HASH_THM; GSYM CONJ_ASSOC] THEN
+gl
+    ENSURES_INIT_TAC "s56" THEN
+    ARM_STEPS_TAC EXEC (57--62) THEN
+    ARM_SUBROUTINE_SIM_TAC
+      (SPEC_ALL a_mc, EXEC, 0, SPEC_ALL a_mc, REWRITE_RULE [num_bytes_per_block; msg_block_at] MSG_SCHEDULE)
+      [`sp + word 80 : int64 `;`m_p : int64`;`m : num -> int64`;
+        `pc : num`; `pc + 0xf8 : num`; `K_base : num`] 63 THEN
+    RENAME_TAC `s63:armstate` `s62:armstate` THEN
+    RULE_ASSUM_TAC (REWRITE_RULE [msg_schedule_at]) THEN
+    RULE_ASSUM_TAC(CONV_RULE (ONCE_DEPTH_CONV EXPAND_CASES_CONV)) THEN
+    RULE_ASSUM_TAC(CONV_RULE (ONCE_DEPTH_CONV NUM_MULT_CONV)) THEN
+    ARM_STEPS_TAC EXEC (63--64) THEN
+    FIRST_X_ASSUM MP_TAC THEN COND_CASES_TAC THENL
+    
+    (* Case: jump *)
+      STRIP_TAC THEN
+      ARM_STEPS_TAC EXEC (139--149) THEN
+      ARM_STEPS_TAC EXEC (73--80) THEN
+      ENSURES_FINAL_STATE_TAC THEN
+      ONCE_ASM_REWRITE_TAC [compression_until] THEN
+      ASM_REWRITE_TAC[LT; msg_schedule_at; ARITH] THEN
 
+      CONJ_TAC THENL
+      [ CHEAT_TAC;???
+        CONV_TAC EXPAND_CASES_CONV THEN
+        CONV_TAC (ONCE_DEPTH_CONV NUM_MULT_CONV) THEN
+        ASM_REWRITE_TAC [] ]
 
+      (* Case: no jump *)
+      STRIP_TAC THEN
+      ARM_STEPS_TAC EXEC (65--79) THEN
+      ARM_STEPS_TAC EXEC [86] THEN
+      ENSURES_FINAL_STATE_TAC THEN
+      ONCE_ASM_REWRITE_TAC [compression_until] THEN
+      ASM_REWRITE_TAC[LT; msg_schedule_at; ARITH] THEN
 
+      CONJ_TAC THENL
+      [ CHEAT_TAC;???
+        CONV_TAC EXPAND_CASES_CONV THEN
+        CONV_TAC (ONCE_DEPTH_CONV NUM_MULT_CONV) THEN
+        ASM_REWRITE_TAC [] ]
 
+    (* Subgoal 3: loop body *)
+    REPEAT STRIP_TAC THEN
+    REWRITE_TAC [hash_buffer_at; EXPAND_HASH_THM; GSYM CONJ_ASSOC] THEN
+    ENSURES_INIT_TAC "s86" THEN
+    RULE_ASSUM_TAC (REWRITE_RULE [msg_schedule_at]) THEN
+    RULE_ASSUM_TAC(CONV_RULE (ONCE_DEPTH_CONV EXPAND_CASES_CONV)) THEN
+    RULE_ASSUM_TAC(CONV_RULE (ONCE_DEPTH_CONV NUM_MULT_CONV)) THEN
+    ARM_STEPS_TAC EXEC (87--117) THEN
+    SUBGOAL_THEN `~(val ((word (i + 1) : int64) + word 18446744073709551536) = 0)`
+      MP_TAC THENL
+      [ REWRITE_TAC[VAL_EQ_0] THEN
+          REWRITE_TAC[WORD_RULE `word_add x y = word 0 <=> x = word_neg y`] THEN
+          CONV_TAC WORD_REDUCE_CONV THEN
+          REWRITE_TAC[GSYM VAL_EQ] THEN
+          VAL_INT64_TAC `i + 1` THEN
+          ASM_REWRITE_TAC[] THEN
+          CONV_TAC WORD_REDUCE_CONV THEN
+          ASM_SIMP_TAC[ARITH_RULE `i < 79 ==> ~(i + 1 = 80)`];
+        DISCH_THEN (fun th -> RULE_ASSUM_TAC (REWRITE_RULE [th])) ]
+    ARM_STEPS_TAC EXEC (81--85) THEN
+    ARM_STEPS_TAC EXEC [87] THEN
+    RENAME_TAC `s87:armstate` `s86':armstate` THEN
+    ENSURES_FINAL_STATE_TAC THEN
+    ASM_REWRITE_TAC[LT; msg_schedule_at; ARITH; WORD_ADD] THEN
+    todo: need to express compression_until i+1 in terms of compression_until i 
+    rewrite with that and solve the msg_schedule_at with the following tactics
+      CONV_TAC EXPAND_CASES_CONV THEN
+      CONV_TAC (ONCE_DEPTH_CONV NUM_MULT_CONV) THEN
+      ASM_REWRITE_TAC []
 
+(* Subgoal 4: backedge *)
+  REPEAT STRIP_TAC THEN ARM_SIM_TAC EXEC []
 
+(* After the loop *)
+ENSURES_INIT_TAC "s86" THEN
+ARM_STEPS_TAC EXEC (87--117) THEN
+rewrite cond, won't branch back
+ARM_STEPS_TAC EXEC (118--138) THEN
+ENSURES_FINAL_STATE_TAC
 
 (*
 (* void sha512_process_blocks(uint64_t h[8], const uint8_t *in_data, size_t num_blocks) *)
-g `! h_p h m_p m l pc retpc K sp.
+g `! h_p h m_p m l pc retpc K_base sp.
   PAIRWISE nonoverlapping
     [(word pc : int64, 2748); (h_p, 640); (m_p, num_bytes_per_block * l);
     (word sp : int64, 768)] ==>
     ensures arm
-    (\s. aligned_bytes_loaded s (word pc) (a_mc pc K) /\
+    (\s. aligned_bytes_loaded s (word pc) (a_mc pc K_base) /\
          read PC s = word pc + ???/\
          read X30 s = retpc /\
          aligned 16 (word sp : int64) /\
@@ -1338,12 +1081,12 @@ g `! h_p h m_p m l pc retpc K sp.
 
 (* void sha512_update(sha512_ctx *sha, const void *in_data, size_t in_len) *)
 g `! ctx_p (h : hash_t) (msg_len_lo : int64) (msg_len_hi : int64) (cur_block : byte list) (cur_pos : byte) (ctx_p : int64)
-     m0 m_p m l pc retpc K sp.
+     m0 m_p m l pc retpc K_base sp.
     nonoverlapping pc, h_p, m_p, stack??? ==>
     LENGTH m = l ==>
     sha512_ctx_inv m0 msg_len_lo msg_len_hi cur_block ==>
     ensures arm
-    (\s. aligned_bytes_loaded s (word pc) (a_mc pc K) /\
+    (\s. aligned_bytes_loaded s (word pc) (a_mc pc K_base) /\
          read PC s = word pc + ??? /\
          read X30 s = retpc /\
          aligned 16 (word sp : int64) /\
@@ -1361,11 +1104,11 @@ g `! ctx_p (h : hash_t) (msg_len_lo : int64) (msg_len_hi : int64) (cur_block : b
 
 (* void sha512_final(uint8_t out[SHA512_DIGEST_LENGTH], sha512_ctx *sha) *)
 g `! ctx_p (h : hash_t) (msg_len_lo : int64) (msg_len_hi : int64) (cur_block : byte list) (cur_pos : byte) (ctx_p : int64)
-     m out_p pc retpc K sp.
+     m out_p pc retpc K_base sp.
     nonoverlapping pc, out_p, stack??? ==>
     sha512_ctx_inv m msg_len_lo msg_len_hi cur_block ==>
     ensures arm
-    (\s. aligned_bytes_loaded s (word pc) (a_mc pc K) /\
+    (\s. aligned_bytes_loaded s (word pc) (a_mc pc K_base) /\
          read PC s = word pc + ??? /\
          read X30 s = retpc /\
          aligned 16 (word sp : int64) /\
